lib/Coqlib_linker.v
@@ -7,3 +7,13 @@ Definition is_empty (X:Type) (l:list X): bool :=
     | nil => true
     | _ => false
   end.
+
+Lemma list_forall2_rev (X Y:Type) (P: X -> Y -> Prop)
+      (lx: list X) (ly: list Y) (H: list_forall2 P lx ly):
+  list_forall2 P (rev lx) (rev ly).
+Proof.
+  generalize dependent ly. induction lx; intros; inv H.
+  { constructor. }
+  simpl. apply list_forall2_app; auto.
+  repeat constructor; auto.
+Qed.
